more notation consistency fixes

Semantics/Imp/Aexp.lean
@@ -5,22 +5,22 @@ namespace Natural
 
 private inductive step: Aexp × State → Int → Prop
   | valₙ: step (val₁ n, _) n
-  | varₙ: step (var₁ x, s) (s x)
-  | addₙ (ha: step (a, s) n) (hb: step (b, s) m):
-    step (a + b, s) (n + m)
-  | subₙ (ha: step (a, s) n) (hb: step (b, s) m):
-    step (a - b, s) (n - m)
-  | mulₙ (ha: step (a, s) n) (hb: step (b, s) m):
-    step (a * b, s) (n * m)
+  | varₙ: step (var₁ v, s) (s v)
+  | addₙ (ha₁: step (a₁, s) n₁) (ha₂: step (a₂, s) n₂):
+    step (a₁ + a₂, s) (n₁ + n₂)
+  | subₙ (ha₁: step (a₁, s) n₁) (ha₂: step (a₂, s) n₂):
+    step (a₁ - a₂, s) (n₁ - n₂)
+  | mulₙ (ha₁: step (a₁, s) n₁) (ha₂: step (a₂, s) n₂):
+    step (a₁ * a₂, s) (n₁ * n₂)
 
 infix:10 " ⟹ₐ " => step
 
 private instance step.equiv: Setoid Aexp where
-  r a b := ∀s n, ((a, s) ⟹ₐ n) = ((b, s) ⟹ₐ n)
+  r a₁ a₂ := ∀s n, ((a₁, s) ⟹ₐ n) = ((a₂, s) ⟹ₐ n)
   iseqv := {
     refl := λ _ _ _ => rfl
     symm := λ h s n => (h s n).symm
-    trans := λ h1 h2 s n => (h1 s n) ▸ (h2 s n)
+    trans := λ h₁ h₂ s n => (h₁ s n) ▸ (h₂ s n)
   }
 
 end Natural
@@ -29,40 +29,42 @@ def reduce (a: Aexp) (s: State): Int :=
   match a with
   | val₁ a => a
   | var₁ a => s a
-  | add₁ a b => reduce a s + reduce b s
-  | sub₁ a b => reduce a s - reduce b s
-  | mul₁ a b => reduce a s * reduce b s
+  | add₁ a₁ a₂ => a₁.reduce s + a₂.reduce s
+  | sub₁ a₁ a₂ => a₁.reduce s - a₂.reduce s
+  | mul₁ a₁ a₂ => a₁.reduce s * a₂.reduce s
 
-instance: CoeFun Aexp (λ _ => State → Int) where
-  coe a := reduce a
+instance: CoeFun Aexp (λ _ => State → Int) := ⟨reduce⟩
 
 instance reduce.equiv: Setoid Aexp where
-  r a b := ∀s, a s = b s
+  r a₁ a₂ := ∀s, a₁ s = a₂ s
   iseqv := {
     refl := λ _ _ => rfl
     symm := λ h s => (h s).symm
-    trans := λ h1 h2 s => (h1 s) ▸ (h2 s)
+    trans := λ h₁ h₂ s => (h₁ s) ▸ (h₂ s)
   }
 
 section Equivalence
 
 -- relational definition is equal to recursive
 private theorem reduce.from_natural
-  (h: p ⟹ₐ n): p.1 p.2 = n :=
-  by induction h with
-  | addₙ _ _ iha ihb => exact iha ▸ ihb ▸ rfl
-  | subₙ _ _ iha ihb => exact iha ▸ ihb ▸ rfl
-  | mulₙ _ _ iha ihb => exact iha ▸ ihb ▸ rfl
+  (hstep: conf ⟹ₐ n): conf.1 conf.2 = n :=
+  by induction hstep with
+  | addₙ _ _ iha₁ iha₂ => exact iha₁ ▸ iha₂ ▸ rfl
+  | subₙ _ _ iha₁ iha₂ => exact iha₁ ▸ iha₂ ▸ rfl
+  | mulₙ _ _ iha₁ iha₂ => exact iha₁ ▸ iha₂ ▸ rfl
   | _ => rfl
 
-private theorem Natural.from_reduce {a: Aexp}
-  (h: a s = n): (a, s) ⟹ₐ n :=
+private theorem Natural.from_reduce
+  (hred: a s = n): (a, s) ⟹ₐ n :=
   by induction a generalizing n with
-  | val₁ a => exact h ▸ step.valₙ
-  | var₁ a => exact h ▸ step.varₙ
-  | add₁ a b iha ihb => exact h ▸ step.addₙ (iha rfl) (ihb rfl)
-  | sub₁ a b iha ihb => exact h ▸ step.subₙ (iha rfl) (ihb rfl)
-  | mul₁ a b iha ihb => exact h ▸ step.mulₙ (iha rfl) (ihb rfl)
+  | val₁ a => exact hred ▸ step.valₙ
+  | var₁ a => exact hred ▸ step.varₙ
+  | add₁ a₁ a₂ iha₁ iha₂ =>
+    exact hred ▸ step.addₙ (iha₁ rfl) (iha₂ rfl)
+  | sub₁ a₁ a₂ iha₁ iha₂ =>
+    exact hred ▸ step.subₙ (iha₁ rfl) (iha₂ rfl)
+  | mul₁ a₁ a₂ iha₁ iha₂ =>
+    exact hred ▸ step.mulₙ (iha₁ rfl) (iha₂ rfl)
 
 private theorem step_eq_reduce:
   ((a, s) ⟹ₐ n) = (a s = n) :=
@@ -73,11 +75,11 @@ private theorem step_eq_reduce':
   Natural.from_reduce rfl
 
 private theorem step_eq_eq_reduce_eq:
-  Natural.step.equiv.r a b ↔ reduce.equiv.r a b := by
+  Natural.step.equiv.r a₁ a₂ ↔ reduce.equiv.r a₁ a₂ := by
   simp only [Setoid.r, eq_iff_iff]
   constructor
   . intro h s
-    specialize h s $ b s
+    specialize h s (a₂ s)
     rw [step_eq_reduce, step_eq_reduce, eq_self, iff_true] at h
     exact h
   . intro h s _
