Semantics/Imp/Natural.lean
@@ -3,29 +3,29 @@ import Semantics.Imp.Bexp
 namespace Com
 namespace Natural
 
-inductive step: Com × State → State → Prop
+inductive step: Config → State → Prop
   | skipₙ:
     step (skip₁, s) s
 
   | assₙ:
-    step (ass₁ x a, s) (s[x ← a s])
+    step (ass₁ v a, s) (s[v ← a s])
 
-  | catₙ (t: State) (hc: step (c, s) t) (hd: step (d, t) u):
-    step (c++d, s) u
+  | catₙ (s₂: State) (hc₁: step (c₁, s₁) s₂) (hc₂: step (c₂, s₂) s₃):
+    step (c₁++c₂, s₁) s₃
 
-  | if₀ₙ {b: Bexp} (hb: b s = false) (hd: step (d, s) t):
-    step (if b then c else d end, s) t
+  | if₀ₙ (hb: b s₁ = false) (hc₂: step (c₂, s₁) s₂):
+    step (if b then c₁ else c₂ end, s₁) s₂
 
-  | if₁ₙ {b: Bexp} (hb: b s = true) (hc: step (c, s) t):
-    step (if b then c else d end, s) t
+  | if₁ₙ (hb: b s₁ = true) (hc₁: step (c₁, s₁) s₂):
+    step (if b then c₁ else c₂ end, s₁) s₂
 
-  | while₀ₙ {b: Bexp} (hb: b s = false):
-    step (while b loop c end, s) s
+  | while₀ₙ (hb: b s₁ = false):
+    step (while b loop c end, s₁) s₁
 
-  | while₁ₙ {b: Bexp}
-    (u: State) (hb: b s = true) (hc: step (c, s) u)
-    (hw: step (while b loop c end, u) t):
-    step (while b loop c end, s) t
+  | while₁ₙ
+    (s₂: State) (hb: b s₁ = true) (hc: step (c, s₁) s₂)
+    (hw: step (while b loop c end, s₂) s₃):
+    step (while b loop c end, s₁) s₃
 
 infix:10 " ⟹ " => step
 
@@ -47,54 +47,54 @@ private example:
 -/
 
 theorem skip_eq:
-  ((skip₁, s) ⟹ t) = (s = t) :=
+  ((skip₁, s₁) ⟹ s₂) = (s₁ = s₂) :=
   propext {
     mp := λ (step.skipₙ) => rfl,
     mpr := (· ▸ step.skipₙ)
   }
 
 theorem cat_eq:
-  ((c++d, s) ⟹ t) = ∃w, ((c, s) ⟹ w) ∧ ((d, w) ⟹ t) :=
+  ((c₁++c₂, s₁) ⟹ s₃) = ∃s₂, ((c₁, s₁) ⟹ s₂) ∧ ((c₂, s₂) ⟹ s₃) :=
   propext {
-    mp := λ (step.catₙ t h1 h2) => ⟨t, h1, h2⟩,
-    mpr := λ ⟨w, h1, h2⟩ => step.catₙ w h1 h2
+    mp := λ (step.catₙ s₂ h₁ h₂) => ⟨s₂, h₁, h₂⟩,
+    mpr := λ ⟨s₂, h₁, h₂⟩ => step.catₙ s₂ h₁ h₂
   }
 
 theorem if_eq:
-  ((if b then c else d end, s) ⟹ t)
-    = bif b s then (c, s) ⟹ t else (d, s) ⟹ t :=
+  ((if b then c₁ else c₂ end, s₁) ⟹ s₂)
+    = bif b s₁ then (c₁, s₁) ⟹ s₂ else (c₂, s₁) ⟹ s₂ :=
   propext {
-    mp := λ h => match h with
+    mp := λ hmp => match hmp with
       | step.if₁ₙ hb h | step.if₀ₙ hb h => hb ▸ h,
-    mpr := match hb: b s with
-      | true => λ h => step.if₁ₙ hb h
-      | false => λ h => step.if₀ₙ hb h
+    mpr := match hb: b s₁ with
+      | true => λ hmp => step.if₁ₙ hb hmp
+      | false => λ hmp => step.if₀ₙ hb hmp
   }
 
 theorem if_eq':
-  ((if b then c else d end, s) ⟹ t)
-    = ((bif b s then c else d, s) ⟹ t) :=
-  propext $ {
-    mp := λ h => match h with
+  ((if b then c₁ else c₂ end, s₁) ⟹ s₂)
+    = ((bif b s₁ then c₁ else c₂, s₁) ⟹ s₂) :=
+  propext {
+    mp := λ hmp => match hmp with
       | step.if₁ₙ hb h | step.if₀ₙ hb h => hb ▸ h,
-    mpr := match hb: b s with
-      | true => λ h => step.if₁ₙ hb h
-      | false => λ h => step.if₀ₙ hb h
+    mpr := match hb: b s₁ with
+      | true => λ hmp => step.if₁ₙ hb hmp
+      | false => λ hmp => step.if₀ₙ hb hmp
   }
 
 theorem while_eq:
-  ((while b loop c end, s) ⟹ t) =
-    bif b s then
-      ∃w, ((c, s) ⟹ w) ∧ ((while b loop c end, w) ⟹ t)
+  ((while b loop c end, s₁) ⟹ s₃) =
+    bif b s₁ then
+      ∃s₂, ((c, s₁) ⟹ s₂) ∧ ((while b loop c end, s₂) ⟹ s₃)
     else
-      s = t :=
+      s₁ = s₃ :=
   propext {
-    mp := λ h => match h with
-      | step.while₁ₙ t hb hc hw => hb ▸ ⟨t, hc, hw⟩
+    mp := λ hmp => match hmp with
+      | step.while₁ₙ s₂ hb hc hw => hb ▸ ⟨s₂, hc, hw⟩
       | step.while₀ₙ hb => hb ▸ rfl,
-    mpr := match hb: b s with
-      | true => λ ⟨w, h1, h2⟩ => step.while₁ₙ w hb h1 h2
-      | false => λ h => h ▸ step.while₀ₙ hb
+    mpr := match hb: b s₁ with
+      | true => λ ⟨s₂, h₁, h₂⟩ => step.while₁ₙ s₂ hb h₁ h₂
+      | false => λ hmp => hmp ▸ step.while₀ₙ hb
   }
 
 /-
@@ -102,7 +102,7 @@ theorem while_eq:
 -/
 
 instance equiv: Setoid Com where
-  r c d := ∀s t, ((c, s) ⟹ t) ↔ ((d, s) ⟹ t)
+  r c₁ c₂ := ∀s₁ s₂, ((c₁, s₁) ⟹ s₂) ↔ ((c₂, s₁) ⟹ s₂)
   iseqv := {
     refl := λ _ _ _ => Iff.rfl
     symm := (Iff.symm $ · · ·)
@@ -123,55 +123,55 @@ theorem skipr:
     mpr := λ h => step.catₙ _ h step.skipₙ
   }
 
-theorem cond_true (h: b ≈ Bexp.true₁):
-  if b then c else d end ≈ c := by
+theorem cond_true (hb: b ≈ Bexp.true₁):
+  if b then c₁ else c₂ end ≈ c₁ := by
   intro _ _
-  rw [if_eq, h]
+  rw [if_eq, hb]
   rfl
 
-theorem cond_false (h: b ≈ Bexp.false₁):
-  if b then c else d end ≈ d := by
+theorem cond_false (hb: b ≈ Bexp.false₁):
+  if b then c₁ else c₂ end ≈ c₂ := by
   intro _ _
-  rw [if_eq, h]
+  rw [if_eq, hb]
   rfl
 
 theorem loop_unfold:
   while b loop c end ≈
     if b then c++while b loop c end else skip₁ end := by
-  intro s t
+  intro s₁ s₃
   rw [if_eq']
   constructor
-  . intro h
-    match h with
-    | step.while₁ₙ w hb hc hw => exact hb ▸ step.catₙ w hc hw
+  . intro hmp
+    match hmp with
+    | step.while₁ₙ s₂ hb hc hw => exact hb ▸ step.catₙ s₂ hc hw
     | step.while₀ₙ hb => exact hb ▸ step.skipₙ
-  . match hb: b s with
+  . match hb: b s₁ with
     | false =>
       intro (step.skipₙ)
       exact step.while₀ₙ hb
     | true =>
-      intro (step.catₙ w hc hw)
-      exact step.while₁ₙ w hb hc hw
+      intro (step.catₙ s₂ hc hw)
+      exact step.while₁ₙ s₂ hb hc hw
 
 /-
 ## Non termination
 -/
 
-theorem loop_tt (h: b ≈ Bexp.true₁):
+theorem loop_tt (htrue: b ≈ Bexp.true₁):
   ¬((while b loop c end, s) ⟹ t) := by
-  intro h1
-  generalize h2: (while b loop c end, s) = p at h1
-  induction h1 generalizing s with
-  | while₁ₙ _ _ _ _ _ ih2 =>
-    match h2 with
-    | Eq.refl _ => exact ih2 rfl
+  intro hmp
+  generalize hconf: (while b loop c end, s) = conf at hmp
+  induction hmp generalizing s with
+  | while₁ₙ _ _ _ _ _ ihw =>
+    match hconf with
+    | Eq.refl _ => exact ihw rfl
   | while₀ₙ hb =>
-    match h2 with
+    match hconf with
     | Eq.refl _ =>
-      rw [h] at hb
+      rw [htrue] at hb
       contradiction
   | _ =>
-    match Prod.mk.injEq _ _ _ _ ▸ h2 with
+    match Prod.mk.injEq _ _ _ _ ▸ hconf with
     | ⟨_, _⟩ => contradiction
 
 /-
@@ -179,39 +179,39 @@ theorem loop_tt (h: b ≈ Bexp.true₁):
 -/
 
 theorem deterministic
-  (hps: p ⟹ s) (hpt: p ⟹ t): s = t :=
-  by induction hps generalizing t with
-  | skipₙ => match hpt with | step.skipₙ => rfl
-  | assₙ => match hpt with | step.assₙ => rfl
-  | catₙ _ _ _ ihc ihd =>
-    match hpt with
-    | step.catₙ _ hc hd =>
-      exact ihd (ihc hc ▸ hd)
-  | if₁ₙ hb _ ih =>
-    match hpt with
-    | step.if₁ₙ _ hd =>
-      exact ih hd
-    | step.if₀ₙ hb1 hd =>
-      rw [hb] at hb1
+  (hps₁: conf ⟹ s₁) (hps₂: conf ⟹ s₂): s₁ = s₂ :=
+  by induction hps₁ generalizing s₂ with
+  | skipₙ => match hps₂ with | step.skipₙ => rfl
+  | assₙ => match hps₂ with | step.assₙ => rfl
+  | catₙ _ _ _ ihc₁ ihc₂ =>
+    match hps₂ with
+    | step.catₙ _ hc₁ hc₂ =>
+      exact ihc₂ (ihc₁ hc₁ ▸ hc₂)
+  | if₁ₙ hb _ ihc₁ =>
+    match hps₂ with
+    | step.if₁ₙ _ hc₁ =>
+      exact ihc₁ hc₁
+    | step.if₀ₙ hb₁ _ =>
+      rw [hb] at hb₁
       contradiction
-  | if₀ₙ hb _ ih =>
-    match hpt with
-    | step.if₁ₙ hb1 _ =>
-      rw [hb] at hb1
+  | if₀ₙ hb _ ihc₂ =>
+    match hps₂ with
+    | step.if₁ₙ hb₁ _ =>
+      rw [hb] at hb₁
       contradiction
     | step.if₀ₙ _ hd =>
-      exact ih hd
+      exact ihc₂ hd
   | while₁ₙ _ hb _ _ ihc ihw =>
-    match hpt with
+    match hps₂ with
     | step.while₁ₙ _ _ hc hw =>
       exact ihw (ihc hc ▸ hw)
-    | step.while₀ₙ hb1 =>
-      rw [hb] at hb1
+    | step.while₀ₙ hb₁ =>
+      rw [hb] at hb₁
       contradiction
   | while₀ₙ hb =>
-    match hpt with
-    | step.while₁ₙ _ hb1 _ _ =>
-      rw [hb] at hb1
+    match hps₂ with
+    | step.while₁ₙ _ hb₁ _ _ =>
+      rw [hb] at hb₁
       contradiction
     | step.while₀ₙ _ => rfl
 
