Semantics/Imp/Structural.lean
@@ -4,18 +4,18 @@ import Semantics.ReflTransRel
 namespace Com
 namespace Structural
 
-inductive step: Com × State → Com × State → Prop where
+inductive step: Config → Config → Prop where
   | assₛ:
-    step (ass₁ x a, s) (skip₁, s[x ← a s])
+    step (ass₁ v a, s) (skip₁, s[v ← a s])
 
   | cat₀ₛ:
     step (skip₁++c, s) (c, s)
 
-  | catₙₛ (h: step (c, s) (e, t)):
-    step (c++d, s) (e++d, t)
+  | catₙₛ (h: step (c₁, s₁) (c₂, s₂)):
+    step (c₁++c₃, s₁) (c₂++c₃, s₂)
 
   | ifₛ:
-    step (if b then c else d end, s) (bif b s then c else d, s)
+    step (if b then c₁ else c₂ end, s) (bif b s then c₁ else c₂, s)
 
   | whileₛ:
     step (while b loop c end, s)
@@ -29,39 +29,39 @@ private example:
   step.catₙₛ step.assₛ
 
 theorem cat_eq:
-  ((c₁++c₂, s) ⇒ et)
-    = ((∃e t, ((c₁, s) ⇒ (e, t)) ∧ et = (e++c₂, t))
-      ∨ (c₁ = skip₁ ∧ et = (c₂, s))) :=
+  ((c₁++c₃, s₁) ⇒ conf)
+    = ((∃c₂ s₂, ((c₁, s₁) ⇒ (c₂, s₂)) ∧ conf = (c₂++c₃, s₂))
+      ∨ (c₁ = skip₁ ∧ conf = (c₃, s₁))) :=
   propext {
-    mp := λ h => match h with
+    mp := λ hmp => match hmp with
       | step.cat₀ₛ => Or.inr ⟨rfl, rfl⟩
       | step.catₙₛ h => Or.inl ⟨_, _, h, rfl⟩,
-    mpr := λ h => match h with
-      | Or.inl ⟨_, _, h1, h2⟩ => h2 ▸ step.catₙₛ h1
-      | Or.inr ⟨h1, h2⟩ => h1 ▸ h2 ▸ step.cat₀ₛ
+    mpr := λ hmpr => match hmpr with
+      | Or.inl ⟨_c₂, _s₂, h₁, h₂⟩ => h₂ ▸ step.catₙₛ h₁
+      | Or.inr ⟨h₁, h₂⟩ => h₁ ▸ h₂ ▸ step.cat₀ₛ
   }
 
 theorem cond_eq:
-  ((if b then c else d end, s) ⇒ ss)
-    = (b s ∧ ss = (c, s) ∨ b s = false ∧ ss = (d, s)) :=
+  ((if b then c₁ else c₂ end, s) ⇒ conf)
+    = (b s ∧ conf = (c₁, s) ∨ b s = false ∧ conf = (c₂, s)) :=
   propext {
-    mp := λ h => match hb: b s with
-      | false => match h with | step.ifₛ => Or.inr ⟨rfl, hb ▸ rfl⟩
-      | true => match h with | step.ifₛ => Or.inl ⟨rfl, hb ▸ rfl⟩,
-    mpr := λ h =>
-      let hss: ss = (bif b s then c else d, s) :=
+    mp := λ hmp => match hb: b s with
+      | false => match hmp with | step.ifₛ => Or.inr ⟨rfl, hb ▸ rfl⟩
+      | true => match hmp with | step.ifₛ => Or.inl ⟨rfl, hb ▸ rfl⟩,
+    mpr := λ hmpr =>
+      let hss: conf = (bif b s then c₁ else c₂, s) :=
         match hb: b s with
-        | true => match hb ▸ h with | Or.inl h => h.2
-        | false => match hb ▸ h with | Or.inr h => h.2
+        | true => match hb ▸ hmpr with | Or.inl ⟨_, h₂⟩ => h₂
+        | false => match hb ▸ hmpr with | Or.inr ⟨_, h₂⟩ => h₂
       hss ▸ step.ifₛ
   }
 
-theorem cond_false {b: Bexp} (hb: b s = false):
-  ((if b then c else d end, s) ⇒ ss) = (ss = (d, s)) :=
+theorem cond_false (hb: b s₁ = false):
+  ((if b then c₁ else c₂ end, s₁) ⇒ conf) = (conf = (c₂, s₁)) :=
   propext {
-    mp := λ h => match hb ▸ cond_eq ▸ h with
-      | Or.inr ⟨_, h2⟩ => h2,
-    mpr := λ h => cond_eq ▸ Or.inr ⟨hb, h⟩
+    mp := λ hmp => match hb ▸ cond_eq ▸ hmp with
+      | Or.inr ⟨_, h₂⟩ => h₂,
+    mpr := λ hmpr => cond_eq ▸ Or.inr ⟨hb, hmpr⟩
   }
 
 infixl:10 " ⇒* " => RTL step
@@ -72,20 +72,20 @@ theorem star.demo₂:
   RTL.head (step.catₙₛ step.assₛ) (RTL.head step.cat₀ₛ RTL.refl)
 
 theorem star.cat_skip_cat
-  (h: (c, s) ⇒* (skip, t)):
-  (c++d, s) ⇒* (skip++d, t) :=
-  RTL.lift (λ (x: Com × State) => (x.1++d, x.2)) (λ _ _ h => step.catₙₛ h) h
+  (hc₁: (c₁, s₁) ⇒* (skip₁, s₂)):
+  (c₁++c₂, s₁) ⇒* (skip₁++c₂, s₂) :=
+  RTL.lift (λ (c₁, s) => (c₁++c₂, s)) (λ _ _ h => step.catₙₛ h) hc₁
 
 theorem star.cat
-  (h1: (c₁, s) ⇒* (skip₁, s₁))
-  (h2: (c₂, s₁) ⇒* (skip₁, s₂)):
-  (c₁++c₂, s) ⇒* (skip₁, s₂) :=
-  RTL.trans (cat_skip_cat h1) (RTL.trans (RTL.single step.cat₀ₛ) h2)
+  (hc₁: (c₁, s₁) ⇒* (skip₁, s₂))
+  (hc₂: (c₂, s₂) ⇒* (skip₁, s₃)):
+  (c₁++c₂, s₁) ⇒* (skip₁, s₃) :=
+  RTL.trans (cat_skip_cat hc₁) (RTL.trans (RTL.single step.cat₀ₛ) hc₂)
 
 theorem star.cat_no_influence
-  (h: (c₁, s) ⇒* (skip₁, s₁)):
+  (hc₁: (c₁, s) ⇒* (skip₁, s₁)):
   (c₁++c₂, s) ⇒* (c₂, s₁) :=
-  RTL.trans (cat_skip_cat h) (RTL.single step.cat₀ₛ)
+  RTL.trans (cat_skip_cat hc₁) (RTL.single step.cat₀ₛ)
 
 end Structural
 end Com
