Semantics/Imp/Equivalence.lean
@@ -5,11 +5,11 @@ import Semantics.Imp.Denotational
 namespace Com
 
 theorem Structural.from_natural
-  (h: p ⟹ s): p ⇒* (skip₁, s) := by
-  induction h with
+  (hconf: conf ⟹ s₂): conf ⇒* (skip₁, s₂) := by
+  induction hconf with
   | skipₙ => exact RTL.refl
   | assₙ => exact RTL.single step.assₛ
-  | catₙ _ _ _ ihc ihd => exact star.cat ihc ihd
+  | catₙ _ _ _ ihc₁ ihc₂ => exact star.cat ihc₁ ihc₂
   | if₁ₙ hb _ ih => exact RTL.head step.ifₛ (hb ▸ ih)
   | if₀ₙ hb _ ih => exact RTL.head step.ifₛ (hb ▸ ih)
   | while₁ₙ _ hb _ _ ihc ihw =>
@@ -18,32 +18,32 @@ theorem Structural.from_natural
     exact RTL.head step.whileₛ $ hb ▸ RTL.refl
 
 theorem Natural.from_structural_step
-  (h₁: x ⇒ y) (h₂: y ⟹ s): x ⟹ s := by
-  induction h₁ generalizing s with
-  | assₛ => exact (skip_eq.mp h₂) ▸ step.assₙ
-  | cat₀ₛ => exact step.catₙ _ step.skipₙ h₂
+  (hconf₁: conf₁ ⇒ conf₂) (hconf₂: conf₂ ⟹ s₂): conf₁ ⟹ s₂ := by
+  induction hconf₁ generalizing s₂ with
+  | assₛ => exact (skip_eq.mp hconf₂) ▸ step.assₙ
+  | cat₀ₛ => exact step.catₙ _ step.skipₙ hconf₂
   | catₙₛ _ ih =>
-    match h₂ with
-    | step.catₙ w hc hd => exact step.catₙ w (ih hc) hd
-  | ifₛ => exact if_eq' ▸ h₂
-  | whileₛ => rw [loop_unfold]; exact if_eq' ▸ h₂
+    match hconf₂ with
+    | step.catₙ s₂ hc₁ hc₂ => exact step.catₙ s₂ (ih hc₁) hc₂
+  | ifₛ => exact if_eq' ▸ hconf₂
+  | whileₛ => rw [loop_unfold]; exact if_eq' ▸ hconf₂
 
 theorem Natural.from_structural
-  (h: x ⇒* (skip₁, t)): x ⟹ t := by
-  induction h using RTL.head_induction_on with
+  (hconf: conf ⇒* (skip₁, s₂)): conf ⟹ s₂ := by
+  induction hconf using RTL.head_induction_on with
   | refl => exact step.skipₙ
-  | head h _ ht => exact from_structural_step h ht
+  | head hsingle _ hs₂ => exact from_structural_step hsingle hs₂
 
 theorem structural_eq_natural:
-  ((c, s) ⇒* (skip₁, t)) = ((c, s) ⟹ t) :=
+  ((c₁, s₁) ⇒* (skip₁, s₂)) = ((c₁, s₁) ⟹ s₂) :=
   propext ⟨Natural.from_structural, Structural.from_natural⟩
 
 theorem denote.from_natural
-  (h: p ⟹ t): (p.2, t) ∈ ⟦p.1⟧ := by
-  induction h with
+  (hconf: conf ⟹ s₃): (conf.2, s₃) ∈ ⟦conf.1⟧ := by
+  induction hconf with
   | skipₙ => exact SFun.mem_id.mpr rfl
   | assₙ  => exact SFun.mem_id.mpr rfl
-  | catₙ t _ _ ih₁ ih₂ => exact ⟨t, ih₁, ih₂⟩
+  | catₙ s₂ _ _ ih₁ ih₂ => exact ⟨s₂, ih₁, ih₂⟩
   | if₁ₙ hb _ ih => exact Or.inl ⟨ih, hb⟩
   | if₀ₙ hb _ ih =>
       apply Or.inr
@@ -51,8 +51,8 @@ theorem denote.from_natural
                   Bool.false_eq_true, not_false_eq_true,
                   and_true]
       exact ih
-  | while₁ₙ t hb _ _ ih₁ ih₂ =>
-    exact while_unfold ▸ Or.inl ⟨⟨t, ih₁, ih₂⟩, hb⟩
+  | while₁ₙ s₂ hb _ _ ih₁ ih₂ =>
+    exact while_unfold ▸ Or.inl ⟨⟨s₂, ih₁, ih₂⟩, hb⟩
   | while₀ₙ hb =>
       rw [while_unfold]
       apply Or.inr
@@ -61,45 +61,46 @@ theorem denote.from_natural
                   and_true]
       rfl
 
-theorem Natural.from_denote (h: (s, t) ∈ ⟦c⟧): (c, s) ⟹ t := by
-  revert h
-  induction c generalizing s t with
+theorem Natural.from_denote
+  (hmem: (s₁, s₃) ∈ ⟦c⟧): (c, s₁) ⟹ s₃ := by
+  revert hmem
+  induction c generalizing s₁ s₃ with
   | skip₁ =>
-    intro h
-    rw [denote, SFun.mem_id] at h
-    exact h ▸ step.skipₙ
+    intro hmp
+    rw [denote, SFun.mem_id] at hmp
+    exact hmp ▸ step.skipₙ
   | ass₁ =>
-    intro h
-    rw [denote.eq_def, Set.mem_comprehend] at h
-    simp only at h
-    exact h ▸ step.assₙ
+    intro hmp
+    rw [denote.eq_def, Set.mem_comprehend] at hmp
+    simp only at hmp
+    exact hmp ▸ step.assₙ
   | cat₁ _ _ ih₁ ih₂ =>
-    intro ⟨w, h1, h2⟩
-    exact step.catₙ w (ih₁ h1) (ih₂ h2)
+    intro ⟨s₂, h₁, h₂⟩
+    exact step.catₙ s₂ (ih₁ h₁) (ih₂ h₂)
   | if₁ _ _ _ ih₁ ih₂ =>
-    intro h
-    match h with
-    | Or.inl ⟨h, hb⟩ =>
-      exact step.if₁ₙ hb (ih₁ h)
-    | Or.inr ⟨h, hb⟩ =>
+    intro hmp
+    match hmp with
+    | Or.inl ⟨h₁, hb⟩ =>
+      exact step.if₁ₙ hb (ih₁ h₁)
+    | Or.inr ⟨h₁, hb⟩ =>
       simp only [Set.mem_comprehend, Bool.not_eq_true] at hb
-      exact step.if₀ₙ hb (ih₂ h)
+      exact step.if₀ₙ hb (ih₂ h₁)
   | while₁ b c ih =>
     suffices
-      ⟦while b loop c end⟧ ⊆ {s | (while b loop c end, s.1) ⟹ s.2} by
+      ⟦while b loop c end⟧ ⊆ {(s₁, s₃) | (while b loop c end, s₁) ⟹ s₃} by
       apply this
 
     apply Fix.lfp_le
-    intro ⟨_, _⟩ h
-    match h with
-    | Or.inl ⟨⟨w, h1, h2⟩, hb⟩ =>
-      exact step.while₁ₙ w hb (ih h1) h2
-    | Or.inr ⟨hq, hb⟩ =>
+    intro ⟨_, _⟩ hmp
+    match hmp with
+    | Or.inl ⟨⟨s₂, h₁, h₂⟩, hb⟩ =>
+      exact step.while₁ₙ s₂ hb (ih h₁) h₂
+    | Or.inr ⟨hid, hb⟩ =>
       simp only [Set.mem_comprehend, Bool.not_eq_true] at hb
-      rw [SFun.mem_id] at hq
-      exact hq ▸ step.while₀ₙ hb
+      rw [SFun.mem_id] at hid
+      exact hid ▸ step.while₀ₙ hb
 
-theorem natural_eq_denote: ((s, t) ∈ ⟦c⟧) = ((c, s) ⟹ t) :=
+theorem natural_eq_denote: ((s₁, s₂) ∈ ⟦c⟧) = ((c, s₁) ⟹ s₂) :=
   propext ⟨Natural.from_denote, denote.from_natural⟩
 
 end Com
