Semantics/Set.lean
@@ -1,58 +1,60 @@
 -- # Sets
 
-def Set (α : Type u) := α → Prop
+def Set (α: Type u) := α → Prop
 
-def setOf {α : Type u} (p : α → Prop) : Set α :=
+def setOf (p: α → Prop): Set α :=
   p
 
 namespace Set
 
-protected def Mem (s : Set α) (a : α) : Prop :=
+protected def Mem (s: Set α) (a: α): Prop :=
   s a
 
-instance : Membership α (Set α) :=
+instance: Membership α (Set α) :=
   ⟨Set.Mem⟩
 
-theorem ext {a b : Set α} (h : ∀ (x : α), x ∈ a ↔ x ∈ b) : a = b :=
-  funext (fun x ↦ propext (h x))
+theorem ext {a b: Set α} (h: ∀ (x: α), x ∈ a ↔ x ∈ b):
+  a = b :=
+  funext (λ x ↦ propext (h x))
 
-protected def Subset (s₁ s₂ : Set α) :=
+protected def Subset (s₁ s₂: Set α) :=
   ∀ ⦃a⦄, a ∈ s₁ → a ∈ s₂
 
-instance : LE (Set α) :=
+instance: LE (Set α) :=
   ⟨Set.Subset⟩
 
-instance : HasSubset (Set α) :=
+instance: HasSubset (Set α) :=
   ⟨(· ≤ ·)⟩
 
-instance : EmptyCollection (Set α) :=
-  ⟨fun _ ↦ False⟩
+instance: EmptyCollection (Set α) :=
+  ⟨λ _ ↦ False⟩
 
 notation (priority := high) "{" x " | " p "}" => setOf (λ x => p)
 
-def univ : Set α := {_a | True}
+def univ: Set α := {_a | True}
 
-protected def insert (a : α) (s : Set α) : Set α := {b | b = a ∨ b ∈ s}
+protected def insert (a: α) (s: Set α): Set α :=
+  {b | b = a ∨ b ∈ s}
 
-instance : Insert α (Set α) := ⟨Set.insert⟩
+instance: Insert α (Set α) := ⟨Set.insert⟩
 
-protected def singleton (a : α) : Set α := {b | b = a}
+protected def singleton (a: α): Set α := {b | b = a}
 
-instance instSingletonSet : Singleton α (Set α) := ⟨Set.singleton⟩
+instance instSingletonSet: Singleton α (Set α) := ⟨Set.singleton⟩
 
-protected def union (s₁ s₂ : Set α) : Set α := {a | a ∈ s₁ ∨ a ∈ s₂}
+protected def union (s₁ s₂: Set α): Set α := {a | a ∈ s₁ ∨ a ∈ s₂}
 
-instance : Union (Set α) := ⟨Set.union⟩
+instance: Union (Set α) := ⟨Set.union⟩
 
-protected def inter (s₁ s₂ : Set α) : Set α := {a | a ∈ s₁ ∧ a ∈ s₂}
+protected def inter (s₁ s₂: Set α): Set α := {a | a ∈ s₁ ∧ a ∈ s₂}
 
-instance : Inter (Set α) := ⟨Set.inter⟩
+instance: Inter (Set α) := ⟨Set.inter⟩
 
-protected def compl (s : Set α) : Set α := {a | a ∉ s}
+protected def compl (s: Set α): Set α := {a | a ∉ s}
 
-protected def diff (s t : Set α) : Set α := {a | a ∈ s ∧ a ∉ t}
+protected def diff (s t: Set α): Set α := {a | a ∈ s ∧ a ∉ t}
 
-instance : SDiff (Set α) := ⟨Set.diff⟩
+instance: SDiff (Set α) := ⟨Set.diff⟩
 
 end Set
 
@@ -60,44 +62,44 @@ end Set
   ## Set theorems
 -/
 
-theorem Set.mem_comprehend {α : Type}
-  (a : α) (P : α → Prop):
-  a ∈ ({a | P a} : Set α) ↔ P a :=
+theorem Set.mem_comprehend
+  (a: α) (P: α → Prop):
+  a ∈ ({a | P a}: Set α) ↔ P a :=
   Iff.rfl
 
-theorem Set.mem_diff {α : Type u} {s t : Set α}
-  (x : α): x ∈ s \ t ↔ x ∈ s ∧ x ∉ t :=
+theorem Set.mem_diff {s t: Set α}
+  (x: α): x ∈ s \ t ↔ x ∈ s ∧ x ∉ t :=
   Iff.rfl
 
 /-
   ### Basic subset properties
 -/
 
-theorem Subset.refl {α : Type}
-  (x : Set α): x ⊆ x :=
+theorem Subset.refl
+  (x: Set α): x ⊆ x :=
   λ _ => id
 
-theorem Subset.trans {α : Type} {x y z : Set α}
-  (h1 : x ⊆ y) (h2 : y ⊆ z) : x ⊆ z :=
-  λ _ h => h2 $ h1 h
+theorem Subset.trans {x y z: Set α}
+  (h₁: x ⊆ y) (h₂: y ⊆ z): x ⊆ z :=
+  λ _ h => h₂ (h₁ h)
 
-theorem Subset.antisymm {α : Type} {x y : Set α}
-  (h1 : x ⊆ y) (h2 : y ⊆ x) : x = y :=
-  funext λ _ => propext ⟨(h1 ·), (h2 ·)⟩
+theorem Subset.antisymm {x y: Set α}
+  (hsub₁: x ⊆ y) (hsub₂: y ⊆ x): x = y :=
+  funext λ _ => propext ⟨(hsub₁ ·), (hsub₂ ·)⟩
 
-theorem Subset.from_eq {α : Type} {x y : Set α}
-  (h : x = y) : x ⊆ y :=
-  λ _ h1 => h ▸ h1
+theorem Subset.from_eq {x y: Set α}
+  (heq: x = y): x ⊆ y :=
+  λ _ h₁ => heq ▸ h₁
 
 /-
   ### Set if then else
 -/
 
-def Set.ite (t s s' : Set α): Set α :=
+def Set.ite (t s s': Set α): Set α :=
   s ∩ t ∪ s' \ t
 
-theorem Set.ite_mono (t : Set α) {s₁ s₁' s₂ s₂' : Set α}
-  (h : s₁ ⊆ s₂) (h' : s₁' ⊆ s₂'):
+theorem Set.ite_mono (t: Set α) {s₁ s₁' s₂ s₂': Set α}
+  (h: s₁ ⊆ s₂) (h': s₁' ⊆ s₂'):
   t.ite s₁ s₁' ⊆ t.ite s₂ s₂' := λ _ h2 =>
   match h2 with
   | Or.inl ⟨hl, hr⟩ => Or.inl ⟨h hl, hr⟩
@@ -127,28 +129,28 @@ theorem mem_comp {f g: α →ˢ α}:
   x ∈ f ○ g ↔ ∃z, (x.1, z) ∈ f ∧ (z, x.2) ∈ g :=
   Iff.rfl
 
-theorem comp_mono {α: Type} {f g h k : Set (α × α)}
-  (hfh : f ⊆ h) (hgk : g ⊆ k): f ○ g ⊆ h ○ k :=
-  λ _ ⟨z, h, h'⟩ => ⟨z, hfh h, hgk h'⟩
+theorem comp_mono {α: Type} {f g h k: Set (α × α)}
+  (hfh: f ⊆ h) (hgk: g ⊆ k): f ○ g ⊆ h ○ k :=
+  λ _ ⟨z, h₁, h₂⟩ => ⟨z, hfh h₁, hgk h₂⟩
 
 theorem comp_id {f: α →ˢ α}: f ○ id = f := by
-  funext x
+  funext (_s₁, s₂)
   apply eq_iff_iff.mpr
   unfold comp
   constructor
-  . intro ⟨z, h1, h2⟩
-    apply mem_id.mp h2 ▸ h1
+  . intro ⟨z, h₁, h₂⟩
+    apply mem_id.mp h₂ ▸ h₁
   . intro h
-    exact ⟨x.2, h, rfl⟩
+    exact ⟨s₂, h, rfl⟩
 
 theorem id_comp {f: α →ˢ α}: id ○ f = f := by
-  funext x
+  funext (s₁, _s₂)
   apply eq_iff_iff.mpr
   unfold comp
   constructor
-  . intro ⟨z, h1, h2⟩
-    apply mem_id.mp h1 ▸ h2
+  . intro ⟨z, h₁, h₂⟩
+    apply mem_id.mp h₁ ▸ h₂
   . intro h
-    exact ⟨x.1, rfl, h⟩
+    exact ⟨s₁, rfl, h⟩
 
 end SFun
